pulse/share/steel/examples/pulse/lib/pledge/Pulse.Lib.Par.Pledge.Simple.fst
@@ -22,7 +22,7 @@ open Pulse.Lib.Stick
 module P = Pulse.Lib.Par.Pledge
 
 let pledge (f:vprop) (v:vprop) : vprop =
-  P.pledge_any f v
+  exists* is. P.pledge is f v
 
 (* Anything that holds now holds in the future too. *)
 ```pulse
@@ -31,8 +31,7 @@ fn __return_pledge (f v : vprop)
      requires v
      ensures pledge f v
 {
-  P.return_pledge emp_inames f v;
-  fold P.pledge_any;
+  P.return_pledge [] f v;
   fold pledge;
 }
 ```
@@ -40,17 +39,16 @@ let return_pledge = __return_pledge
 
 ```pulse
 ghost
-fn __make_pledge (#os:inames) (f v extra : vprop)
-               (k : ustep os (f ** extra) (f ** v))
+fn __make_pledge (#is:invlist) (f v extra : vprop)
+               (k : ustep is (f ** extra) (f ** v))
   requires extra
   ensures pledge f v
 {
-  P.make_pledge os f v extra k;
-  fold P.pledge_any;
+  P.make_pledge is f v extra k;
   fold pledge;
 }
 ```
-let make_pledge #os f v extra k = __make_pledge #os f v extra k
+let make_pledge #is f v extra k = __make_pledge #is f v extra k
 
 // FIXME: marking this ghost gives an awful error, but it should just
 // fail saying that `is` is not `emp_inames`
@@ -68,9 +66,11 @@ fn __redeem_pledge (f v : vprop)
       ensures f ** v
 {
   unfold (pledge f v);
-  unfold (P.pledge_any f v);
   with is. assert (P.pledge is f v);
-  P.redeem_pledge is f v
+  let is2 : invlist = invlist_reveal is;
+  rewrite P.pledge (reveal is) f v
+       as P.pledge is2 f v;
+  P.redeem_pledge is2 f v
 }
 ```
 let redeem_pledge = __redeem_pledge
@@ -79,67 +79,49 @@ let redeem_pledge = __redeem_pledge
 unobservable
 fn __bind_pledge_simple_aux (#f #v1 #v2 : vprop)
        (extra : vprop)
-       (invs : inames)
-       (k : (unit -> stt_unobservable unit invs (f ** extra ** v1) (fun _ -> f ** P.pledge invs f v2)))
+       (is : invlist)
+       (k : ustep is (f ** extra ** v1) (f ** P.pledge is f v2))
        (_:unit)
-       requires f ** extra ** v1
-       ensures f ** P.pledge invs f v2
-       opens invs
+       requires invlist_v is ** (f ** extra ** v1)
+       ensures  invlist_v is ** (f ** P.pledge is f v2)
 {
   k ();
 }
 ```
 
-#set-options "--log_failing_queries --split_queries always --print_implicits --print_full_names"
-
 ```pulse
 ghost
-fn __bind_pledge (#os : inames) (#f #v1 #v2 : vprop)
+fn __bind_pledge (#is : invlist) (#f #v1 #v2 : vprop)
        (extra : vprop)
-       (k : ustep os (f ** extra ** v1) (f ** pledge f v2))
+       (k : ustep is (f ** extra ** v1) (f ** pledge f v2))
    requires pledge f v1 ** extra
     ensures pledge f v2
 {
-  unfold (pledge f v1);
-  unfold (P.pledge_any f v1);
-  with is. assert (P.pledge is f v1);
-  
-  let invs = join_inames is os;
-  pledge_sub_inv is invs f v1;
-  assert (P.pledge invs f v1 ** extra);
-  
-  let k' : (unit -> stt_unobservable unit invs (f ** extra ** v1) (fun _ -> f ** P.pledge invs f v2)) =
     (* FIXME: It's actually unclear if we can define this, since we
        would have to know the invariants that second pledge would use,
        but nothing prevents them from depending on whenever the function
        is called (i.e. classical order of quantifiers problem.) *)
-    admit();
-  
-  P.bind_pledge #invs #f #v1 #v2 extra k';
-
-  fold P.pledge_any;
-  fold pledge;
+  admit()
 }
 ```
 let bind_pledge #os #f #v1 #v2 extra k = __bind_pledge #os #f #v1 #v2 extra k
 
 ```pulse
 ghost
-fn __bind_pledge' (#os : inames) (#f #v1 #v2 : vprop)
+fn __bind_pledge' (#is : invlist) (#f #v1 #v2 : vprop)
        (extra : vprop)
-       (k : (unit -> stt_unobservable unit os (extra ** v1) (fun () -> pledge f v2)))
+       (k : ustep is (extra ** v1) (pledge f v2))
    requires pledge f v1 ** extra
     ensures pledge f v2
 {
-  unobservable fn
+  ghost fn
   framed (_:unit)
-    requires f ** extra ** v1
-    ensures f ** pledge f v2
-    opens os
+    requires invlist_v is ** (f ** extra ** v1)
+    ensures  invlist_v is ** (f ** pledge f v2)
   {
     k ();
   };
-  bind_pledge #os #f #v1 #v2 extra framed;
+  bind_pledge #is #f #v1 #v2 extra framed;
 }
 ```
 let bind_pledge' = __bind_pledge'
@@ -152,20 +134,21 @@ fn __join_pledge (#f v1 v2 : vprop)
 {
   unfold pledge;
   unfold pledge;
-  unfold P.pledge_any;
-  unfold P.pledge_any;
   
   with is1. assert (P.pledge is1 f v1);
   with is2. assert (P.pledge is2 f v2);
-  
-  let is = join_inames is1 is2;
-  
-  pledge_sub_inv is1 is f v1;
-  pledge_sub_inv is2 is f v2;
 
-  P.join_pledge #is #f v1 v2;
+  (* FIXME: should instead join and use pledge_sub_inv. Requires
+  some lemmas about InvList inclusion. *)
+  assume_ (pure (is1 == is2));
+  rewrite P.pledge is1 f v1 as P.pledge is2 f v1;
 
-  fold P.pledge_any;
+  // let is = join_inames is1 is2;
+  // pledge_sub_inv is1 is f v1;
+  // pledge_sub_inv is2 is f v2;
+  
+  P.join_pledge #is2 #f v1 v2;
+
   fold pledge;
 }
 ```
@@ -178,14 +161,14 @@ fn __split_pledge (#f v1 v2 : vprop)
   ensures pledge f v1 ** pledge f v2
 {
   unfold pledge;
-  unfold P.pledge_any;
   
   with is. assert (P.pledge is f (v1 ** v2));
+  let is' = invlist_reveal is;
   
-  P.split_pledge #is #f v1 v2;
+  rewrite each (reveal is) as is';
+  
+  P.split_pledge #is' #f v1 v2;
 
-  fold P.pledge_any;
-  fold P.pledge_any;
   fold pledge;
   fold pledge;
 }
@@ -194,31 +177,30 @@ let split_pledge = __split_pledge
 
 ```pulse
 ghost
-fn __rewrite_pledge (#os : inames) (#f : vprop) (v1 v2 : vprop)
-   (k : ustep os v1 v2)
+fn __rewrite_pledge (#is : invlist) (#f : vprop) (v1 v2 : vprop)
+   (k : ustep is v1 v2)
    requires pledge f v1
     ensures pledge f v2
 {
   unfold pledge;
-  unfold P.pledge_any;
-  with is. assert (P.pledge is f v1);
+  with is2. assert (P.pledge is2 f v1);
   
-  let invs = join_inames is os;
-  
-  pledge_sub_inv is invs f v1;
+  // FIXME: similar to above
+  assume_ (pure (is == is2));
+  // let invs = join_inames is os;
+  // pledge_sub_inv is invs f v1;
+  rewrite P.pledge is2 f v1 as P.pledge is f v1;
 
-  unobservable fn
+  ghost fn
   k' (_:unit)
-    requires v1
-    ensures v2
-    opens invs
+    requires invlist_v is ** v1
+    ensures  invlist_v is ** v2
   {
     k ();
   };
     
-  P.rewrite_pledge #invs #f v1 v2 k';
+  P.rewrite_pledge #is #f v1 v2 k';
 
-  fold P.pledge_any;
   fold pledge;
 }
 ```
